---
title: Draft
date: 2000-01-01 00:00:00
tags:
mathjax: true
top: true
---

草稿

<!--more-->

$\sum \limits_{d \mid n} \mu(d) = [n = 1]$

$\mu * I = e$

---

$\sum \limits_{d \mid n} \varphi(d) = n$

$\varphi(d) * I = id$

---

$\sum \limits_{d \mid n} d \mu(\frac{n}{d}) = \varphi(n)$

$\mu * id = \varphi$

---

$\sum \limits_{d \mid n} \mu(d) = [n = 1]$

$[\gcd(i, j) = 1] = \sum \limits_{d \mid i, d \mid j}\mu(d)$

---

$\sum\limits_{i = 1}^{n} \sum \limits_{j = 1}^{m} \sum \limits_{d \mid i, d \mid j} \mu(d) = \sum \limits_{d = 1}^{n} \mu(d) \lfloor \frac{n}{d} \rfloor \lfloor \frac{m}{d} \rfloor$

---

$B_t(x) \equiv B_{t - 1}(x)(2 - A(x)B_{t - 1}(x)) \pmod{x^{2^t}}$

---

~~$f_i(x) = f(x) \frac{w_i}{x - x_i}$~~

~~$F(x) = f(x)\sum\limits_{i = 0}^n \frac{w_i}{x - x_i} y_i$~~

$P_n(x) = y_i\frac{(x - x2)(x - x3) \cdots (x - x_n)(x - x_{n + 1})}{(x_1 - x_2)(x_1 - x_3)\cdots(x_1 - x_n)(x_1 - x_{n + 1})}$
